@prefix : <http://www.semanticweb.org/research-organization#> .
@prefix owl: <http://www.w3.org/2002/07/owl#> .
@prefix rdf: <http://www.w3.org/1999/02/22-rdf-syntax-ns#> .
@prefix xml: <http://www.w3.org/XML/1998/namespace> .
@prefix xsd: <http://www.w3.org/2001/XMLSchema#> .
@prefix rdfs: <http://www.w3.org/2000/01/rdf-schema#> .
@base <http://www.semanticweb.org/research-organization> .

<http://www.semanticweb.org/research-organization> rdf:type owl:Ontology .

#################################################################
#    Object Properties
#################################################################

###  http://www.semanticweb.org/research-organization#directs
:directs rdf:type owl:ObjectProperty ;
         owl:inverseOf :isDirectedBy ;
         rdf:type owl:InverseFunctionalProperty ;
         rdfs:domain :Director ;
         rdfs:range :Institute ;
         rdfs:comment "directs relates a director to an institute in which they works"@en ;
         rdfs:label "directs"@en .


###  http://www.semanticweb.org/research-organization#hasBuilding
:hasBuilding rdf:type owl:ObjectProperty ;
             rdfs:subPropertyOf :hasPart ;
             owl:inverseOf :isBuildingOf ;
             rdf:type owl:InverseFunctionalProperty ;
             rdfs:domain :Institute ;
             rdfs:range :Building ;
             rdfs:comment "hasBuilding is a subproperty of hasPart and relates institute to the buildings that belongs to it"@en ;
             rdfs:label "has building"@en .


###  http://www.semanticweb.org/research-organization#hasContractWith
:hasContractWith rdf:type owl:ObjectProperty ;
                 owl:inverseOf :makesContractWith ;
                 rdf:type owl:FunctionalProperty ;
                 rdfs:domain :Employee ;
                 rdfs:range :ResearchOrganization ;
                 rdfs:comment "hasContractWith relates an employee to the research organization with which he has a contract"@en ;
                 rdfs:label "has contract with"@en .


###  http://www.semanticweb.org/research-organization#hasInstitute
:hasInstitute rdf:type owl:ObjectProperty ;
              rdfs:subPropertyOf :hasPart ;
              owl:inverseOf :isInstituteOf ;
              rdf:type owl:InverseFunctionalProperty ;
              rdfs:domain :ResearchOrganization ;
              rdfs:range :Institute ;
              rdfs:comment "hasInstitute is a subproperty of hasPart and relates a research organization to the institutes that compose it"@en ;
              rdfs:label "has institute"@en .


###  http://www.semanticweb.org/research-organization#hasLaboratory
:hasLaboratory rdf:type owl:ObjectProperty ;
               rdfs:subPropertyOf :hasPart ;
               owl:inverseOf :isLaboratoryOf ;
               rdf:type owl:InverseFunctionalProperty ;
               rdfs:domain :Institute ;
               rdfs:range :Laboratory ;
               rdfs:comment "hasLaboratory is a subproperty of hasPart and relates an institute to laboratories that compose it"@en ;
               rdfs:label "has laboratory"@en .


###  http://www.semanticweb.org/research-organization#hasLaboratoryMember
:hasLaboratoryMember rdf:type owl:ObjectProperty ;
                     rdfs:subPropertyOf :hasMember ;
                     owl:inverseOf :isMemberOfLaboratory ;
                     rdf:type owl:InverseFunctionalProperty ;
                     rdfs:domain :Laboratory ;
                     rdfs:range [ rdf:type owl:Class ;
                                  owl:unionOf ( :AdministrativeStaff
                                                :GraduateFellow
                                                :PostdoctoralFellow
                                                :Researcher
                                                :Technologist
                                              )
                                ] ;
                     rdfs:comment "hasLaboratoryMember relates a Laboratory with its members. Each member is: graduate fellow or postdoctoral fellow or researcher or technologist or AdministrativeStaff"@en ;
                     rdfs:label "has laboratory member"@en .


###  http://www.semanticweb.org/research-organization#hasLocation
:hasLocation rdf:type owl:ObjectProperty ;
             owl:inverseOf :isLocationOf ;
             rdf:type owl:FunctionalProperty ;
             rdfs:domain :Building ;
             rdfs:range :Location ;
             rdfs:comment "hasLocation relates a building to the location where it is placed"@en ;
             rdfs:label "has location"@en .


###  http://www.semanticweb.org/research-organization#hasMember
:hasMember rdf:type owl:ObjectProperty ;
           owl:inverseOf :isMemberOf ;
           rdf:type owl:ReflexiveProperty ;
           rdfs:comment "hasMember is superproperty of: hasResearchGroupMember, hasLaboratoryMember"@en ;
           rdfs:label "has member"@en .


###  http://www.semanticweb.org/research-organization#hasOffice
:hasOffice rdf:type owl:ObjectProperty ;
           rdfs:subPropertyOf :hasPart ;
           owl:inverseOf :isOfficeOf ;
           rdf:type owl:InverseFunctionalProperty ;
           rdfs:domain :Building ;
           rdfs:range :Office ;
           rdfs:comment "hasOffice is a subproperty of hasPart and relates a building to the offices belonging to it"@en ;
           rdfs:label "has office"@en .


###  http://www.semanticweb.org/research-organization#hasPart
:hasPart rdf:type owl:ObjectProperty ;
         owl:inverseOf :isPartOf ;
         rdf:type owl:TransitiveProperty ,
                  owl:ReflexiveProperty ;
         rdfs:comment "hasPart is a superproperty of: hasInstitute, hasLaboratory, hasResearchGroup, hasBuilding and hasOffice"@en ;
         rdfs:label "has part"@en .


###  http://www.semanticweb.org/research-organization#hasResearchGroup
:hasResearchGroup rdf:type owl:ObjectProperty ;
                  rdfs:subPropertyOf :hasPart ;
                  owl:inverseOf :isResearchGroupOf ;
                  rdf:type owl:InverseFunctionalProperty ;
                  rdfs:domain :Laboratory ;
                  rdfs:range :ResearchGroup ;
                  rdfs:comment "hasResearchGroup is a subproperty of hasPart and relates laboratory with research groups that compose it"@en ;
                  rdfs:label "has research group"@en .


###  http://www.semanticweb.org/research-organization#hasResearchGroupMember
:hasResearchGroupMember rdf:type owl:ObjectProperty ;
                        rdfs:subPropertyOf :hasMember ;
                        owl:inverseOf :isMemberOfResearchGroup ;
                        rdf:type owl:InverseFunctionalProperty ;
                        rdfs:domain :ResearchGroup ;
                        rdfs:range [ rdf:type owl:Class ;
                                     owl:unionOf ( :AdministrativeStaff
                                                   :GraduateFellow
                                                   :PostdoctoralFellow
                                                   :Researcher
                                                   :Technologist
                                                 )
                                   ] ;
                        rdfs:comment "hasResearchGroupMember relates a research group with its members. Each member is: graduate fellow or postdoctoral fellow or researcher or technologist or AdministrativeStaff"@en ;
                        rdfs:label "has research group member"@en .


###  http://www.semanticweb.org/research-organization#hosts
:hosts rdf:type owl:ObjectProperty ;
       owl:inverseOf :isHostedIn ;
       rdf:type owl:InverseFunctionalProperty ;
       rdfs:domain :Office ;
       rdfs:range :Employee ;
       rdfs:comment "hosts relates an office to employees that work in it"@en ;
       rdfs:label "hosts"@en .


###  http://www.semanticweb.org/research-organization#isBuildingOf
:isBuildingOf rdf:type owl:ObjectProperty ;
              rdfs:subPropertyOf :isPartOf ;
              rdf:type owl:FunctionalProperty ;
              rdfs:domain :Building ;
              rdfs:range :Institute ;
              rdfs:comment "isBuildingOf is a subproperty of isPartOf and relates buildings to the institute they belong to"@en ;
              rdfs:label "is building of"@en .


###  http://www.semanticweb.org/research-organization#isDirectedBy
:isDirectedBy rdf:type owl:ObjectProperty ,
                       owl:FunctionalProperty ;
              rdfs:domain :Institute ;
              rdfs:range :Director ;
              rdfs:comment "isDirectedBy relates an institute to director that work in it"@en ;
              rdfs:label "is directed by"@en .


###  http://www.semanticweb.org/research-organization#isHostedIn
:isHostedIn rdf:type owl:ObjectProperty ,
                     owl:FunctionalProperty ;
            rdfs:domain :Employee ;
            rdfs:range :Office ;
            rdfs:comment "isHostedIn relates employees to the office in which they works"@en ;
            rdfs:label "is hosted in"@en .


###  http://www.semanticweb.org/research-organization#isInstituteOf
:isInstituteOf rdf:type owl:ObjectProperty ;
               rdfs:subPropertyOf :isPartOf ;
               rdf:type owl:FunctionalProperty ;
               rdfs:domain :Institute ;
               rdfs:range :ResearchOrganization ;
               rdfs:comment "isIntituteOf is a subproperty of isPartOf and relates intitutes to the research organization of which it is composed"@en ;
               rdfs:label "is institute of"@en .


###  http://www.semanticweb.org/research-organization#isLaboratoryOf
:isLaboratoryOf rdf:type owl:ObjectProperty ;
                rdfs:subPropertyOf :isPartOf ;
                rdf:type owl:FunctionalProperty ;
                rdfs:domain :Laboratory ;
                rdfs:range :Institute ;
                rdfs:comment "isLaboratoryOf is a subproperty of isPartOf and relates laboratories to the institute of which it is composed"@en ;
                rdfs:label "is laboratory of"@en .


###  http://www.semanticweb.org/research-organization#isLocationOf
:isLocationOf rdf:type owl:ObjectProperty ,
                       owl:InverseFunctionalProperty ;
              rdfs:domain :Location ;
              rdfs:range :Building ;
              rdfs:comment "isLocationOf relates a location to buildings that are placed there"@en ;
              rdfs:label "is location of"@en .


###  http://www.semanticweb.org/research-organization#isMemberOf
:isMemberOf rdf:type owl:ObjectProperty ,
                     owl:ReflexiveProperty ;
            rdfs:comment "isMemberOf is a superproperty of: isMemberOfLaboratory and isMemberOfResearchGroup"@en ;
            rdfs:label "is member of"@en .


###  http://www.semanticweb.org/research-organization#isMemberOfLaboratory
:isMemberOfLaboratory rdf:type owl:ObjectProperty ;
                      rdfs:subPropertyOf :isMemberOf ;
                      rdf:type owl:FunctionalProperty ;
                      rdfs:domain [ rdf:type owl:Class ;
                                    owl:unionOf ( :AdministrativeStaff
                                                  :GraduateFellow
                                                  :PostdoctoralFellow
                                                  :Researcher
                                                  :Technologist
                                                )
                                  ] ;
                      rdfs:range :Laboratory ;
                      rdfs:comment "isMemberOfLaboratory is a subproperty of isMember and relates the members of a reserach group to their research group. Each member is: graduate fellow or postdoctoral fellow or researcher or technologist or AdministrativeStaff"@en ;
                      rdfs:label "is member of laboratory"@en .


###  http://www.semanticweb.org/research-organization#isMemberOfResearchGroup
:isMemberOfResearchGroup rdf:type owl:ObjectProperty ;
                         rdfs:subPropertyOf :isMemberOf ;
                         rdf:type owl:FunctionalProperty ;
                         rdfs:domain [ rdf:type owl:Class ;
                                       owl:unionOf ( :AdministrativeStaff
                                                     :GraduateFellow
                                                     :PostdoctoralFellow
                                                     :Researcher
                                                     :Technologist
                                                   )
                                     ] ;
                         rdfs:range :ResearchGroup ;
                         rdfs:comment "isMemberOfResearchGroup is a subproperty of isMember and relates the members of a reserach group to their research group. Each member is: graduate fellow or postdoctoral fellow or researcher or technologist or AdministrativeStaff"@en ;
                         rdfs:label "is member of research group"@en .


###  http://www.semanticweb.org/research-organization#isOfficeOf
:isOfficeOf rdf:type owl:ObjectProperty ;
            rdfs:subPropertyOf :isPartOf ;
            rdf:type owl:FunctionalProperty ;
            rdfs:domain :Office ;
            rdfs:range :Building ;
            rdfs:comment "isOfficeOf is a subproperty of isPartOf and relates offices to the building they belong to"@en ;
            rdfs:label "is office of"@en .


###  http://www.semanticweb.org/research-organization#isPartOf
:isPartOf rdf:type owl:ObjectProperty ,
                   owl:TransitiveProperty ,
                   owl:ReflexiveProperty ;
          rdfs:comment "isPartOf is a superproperty of:  isOfficeOf, isBuildingOf, isInstituteOf, isLaboratoryOf, and isResearchGroupOf"@en ;
          rdfs:label "is part of"@en .


###  http://www.semanticweb.org/research-organization#isResearchGroupOf
:isResearchGroupOf rdf:type owl:ObjectProperty ;
                   rdfs:subPropertyOf :isPartOf ;
                   rdf:type owl:FunctionalProperty ;
                   rdfs:domain :ResearchGroup ;
                   rdfs:range :Laboratory ;
                   rdfs:comment "isResearchGroupOf is a subproperty of isPartOf and relates research groups to the laboratory of which it is composed"@en ;
                   rdfs:label "is research group of"@en .


###  http://www.semanticweb.org/research-organization#makesContractWith
:makesContractWith rdf:type owl:ObjectProperty ,
                            owl:InverseFunctionalProperty ;
                   rdfs:domain :ResearchOrganization ;
                   rdfs:range :Employee ;
                   rdfs:comment "makesContracWith relates a research organization to employees that have a contract with it"@en ;
                   rdfs:label "makes contract with"@en .


#################################################################
#    Data properties
#################################################################

###  http://www.semanticweb.org/research-organization#hasDate
:hasDate rdf:type owl:DatatypeProperty ,
                  owl:FunctionalProperty ;
         rdfs:domain :Institute ;
         rdfs:range xsd:dateTime ;
         rdfs:comment "hasDate relates a institute and the date of its creation"@en ;
         rdfs:label "has date"@en .


###  http://www.semanticweb.org/research-organization#hasEmployeeID
:hasEmployeeID rdf:type owl:DatatypeProperty ;
               rdfs:subPropertyOf :hasID ;
               rdf:type owl:FunctionalProperty ;
               rdfs:domain :Employee ;
               rdfs:range xsd:positiveInteger ;
               owl:propertyDisjointWith :hasInstituteID ;
               rdfs:comment "hasEmployeeID is a subproperty of hasID and relates an employee with his ID that is an integer"@en ;
               rdfs:label "has employee ID"@en .


###  http://www.semanticweb.org/research-organization#hasID
:hasID rdf:type owl:DatatypeProperty ;
       rdfs:comment "hasID is a superproperty of: hasEmployeeID and hasInstituteID"@en ;
       rdfs:label "has ID"@en .


###  http://www.semanticweb.org/research-organization#hasInstituteID
:hasInstituteID rdf:type owl:DatatypeProperty ;
                rdfs:subPropertyOf :hasID ;
                rdf:type owl:FunctionalProperty ;
                rdfs:domain :Institute ;
                rdfs:range xsd:positiveInteger ;
                rdfs:comment "hasInstituteID is a subproperty of hasID and relates an institute with his ID that is an integer"@en ;
                rdfs:label "has institute ID"@en .


###  http://www.semanticweb.org/research-organization#hasInstituteName
:hasInstituteName rdf:type owl:DatatypeProperty ;
                  rdfs:subPropertyOf :hasName ;
                  rdf:type owl:FunctionalProperty ;
                  rdfs:domain :Institute ;
                  rdfs:range xsd:string ;
                  rdfs:comment "hasIntituteName is a subproperty of hasName and relates an institute to its name that is a string"@en ;
                  rdfs:label "has institute name"@en .


###  http://www.semanticweb.org/research-organization#hasLaboratoryName
:hasLaboratoryName rdf:type owl:DatatypeProperty ;
                   rdfs:subPropertyOf :hasName ;
                   rdf:type owl:FunctionalProperty ;
                   rdfs:domain :Laboratory ;
                   rdfs:range xsd:string ;
                   rdfs:comment "hasLaboratoryName is a subproperty of hasName and relates a laboratory to its name that is a string"@en ;
                   rdfs:label "has laboratory name"@en .


###  http://www.semanticweb.org/research-organization#hasName
:hasName rdf:type owl:DatatypeProperty ;
         rdfs:comment "hasName is a superproperty of: hasInstituteName, hasLaboratoryName and hasResearchGroupName"@en ;
         rdfs:label "has name"@en .


###  http://www.semanticweb.org/research-organization#hasResearchGroupName
:hasResearchGroupName rdf:type owl:DatatypeProperty ;
                      rdfs:subPropertyOf :hasName ;
                      rdf:type owl:FunctionalProperty ;
                      rdfs:domain :ResearchGroup ;
                      rdfs:range xsd:string ;
                      rdfs:comment "hasResearchGroupName is a subproperty of hasName and relates a research group to its name that is a string"@en ;
                      rdfs:label "has research group name"@en .


#################################################################
#    Classes
#################################################################

###  http://www.semanticweb.org/research-organization#AdministrativeStaff
:AdministrativeStaff rdf:type owl:Class ;
                     rdfs:subClassOf :Employee ,
                                     [ rdf:type owl:Restriction ;
                                       owl:onProperty :isMemberOfLaboratory ;
                                       owl:qualifiedCardinality "1"^^xsd:nonNegativeInteger ;
                                       owl:onClass :Laboratory
                                     ] ,
                                     [ rdf:type owl:Restriction ;
                                       owl:onProperty :isMemberOfResearchGroup ;
                                       owl:qualifiedCardinality "1"^^xsd:nonNegativeInteger ;
                                       owl:onClass :ResearchGroup
                                     ] ;
                     rdfs:comment "An AdministrativeStaff is an employee that is member of exactly one laboratory and research group" ;
                     rdfs:label "administrative staff" .


###  http://www.semanticweb.org/research-organization#Building
:Building rdf:type owl:Class ;
          rdfs:subClassOf [ rdf:type owl:Restriction ;
                            owl:onProperty :hasOffice ;
                            owl:someValuesFrom :Office
                          ] ,
                          [ rdf:type owl:Restriction ;
                            owl:onProperty :hasLocation ;
                            owl:qualifiedCardinality "1"^^xsd:nonNegativeInteger ;
                            owl:onClass :Location
                          ] ;
          rdfs:comment "A Building is a structure, an edifice that has a location and some offices"@en ;
          rdfs:label "building"@en .


###  http://www.semanticweb.org/research-organization#Director
:Director rdf:type owl:Class ;
          rdfs:subClassOf :Researcher ;
          rdfs:comment "A director is a person that is an Employee and a Researcher"@en ;
          rdfs:label "director"@en .


###  http://www.semanticweb.org/research-organization#Employee
:Employee rdf:type owl:Class ;
          rdfs:subClassOf <http://xmlns.com/foaf/0.1/Person> ,
                          [ rdf:type owl:Restriction ;
                            owl:onProperty :hasContractWith ;
                            owl:qualifiedCardinality "1"^^xsd:nonNegativeInteger ;
                            owl:onClass :ResearchOrganization
                          ] ,
                          [ rdf:type owl:Restriction ;
                            owl:onProperty :isHostedIn ;
                            owl:qualifiedCardinality "1"^^xsd:nonNegativeInteger ;
                            owl:onClass :Office
                          ] ,
                          [ rdf:type owl:Restriction ;
                            owl:onProperty :hasEmployeeID ;
                            owl:allValuesFrom xsd:positiveInteger
                          ] ,
                          [ rdf:type owl:Restriction ;
                            owl:onProperty :hasEmployeeID ;
                            owl:qualifiedCardinality "1"^^xsd:nonNegativeInteger ;
                            owl:onDataRange xsd:positiveInteger
                          ] ;
          rdfs:comment "An Employee is a person who has a contract with the research organization and has an office. An Employee can be a graduate or postdoctoral fellow, a researcher (young, senior or director), a technologist."@en ;
          rdfs:label "employee"@en .


###  http://www.semanticweb.org/research-organization#GraduateFellow
:GraduateFellow rdf:type owl:Class ;
                rdfs:subClassOf :Employee ,
                                [ rdf:type owl:Restriction ;
                                  owl:onProperty :isMemberOfLaboratory ;
                                  owl:qualifiedCardinality "1"^^xsd:nonNegativeInteger ;
                                  owl:onClass :Laboratory
                                ] ,
                                [ rdf:type owl:Restriction ;
                                  owl:onProperty :isMemberOfResearchGroup ;
                                  owl:qualifiedCardinality "1"^^xsd:nonNegativeInteger ;
                                  owl:onClass :ResearchGroup
                                ] ;
                rdfs:comment "An GraduateFellow is an employee that is member of exactly one laboratory and research group"@en ;
                rdfs:label "graduate fellow"@en .


###  http://www.semanticweb.org/research-organization#Institute
:Institute rdf:type owl:Class ;
           rdfs:subClassOf [ rdf:type owl:Restriction ;
                             owl:onProperty :hasBuilding ;
                             owl:someValuesFrom :Building
                           ] ,
                           [ rdf:type owl:Restriction ;
                             owl:onProperty :hasLaboratory ;
                             owl:someValuesFrom :Laboratory
                           ] ,
                           [ rdf:type owl:Restriction ;
                             owl:onProperty :isDirectedBy ;
                             owl:qualifiedCardinality "1"^^xsd:nonNegativeInteger ;
                             owl:onClass :Director
                           ] ,
                           [ rdf:type owl:Restriction ;
                             owl:onProperty :hasDate ;
                             owl:qualifiedCardinality "1"^^xsd:nonNegativeInteger ;
                             owl:onDataRange xsd:dateTime
                           ] ,
                           [ rdf:type owl:Restriction ;
                             owl:onProperty :hasInstituteID ;
                             owl:qualifiedCardinality "1"^^xsd:nonNegativeInteger ;
                             owl:onDataRange xsd:positiveInteger
                           ] ,
                           [ rdf:type owl:Restriction ;
                             owl:onProperty :hasInstituteName ;
                             owl:qualifiedCardinality "1"^^xsd:nonNegativeInteger ;
                             owl:onDataRange xsd:string
                           ] ;
           rdfs:comment "An Institute is part of a research organization. Each Institute has a name and an ID, is directed by exactly one director, has buildings and consists of more than one laboratory."@en ;
           rdfs:label "institute"@en .


###  http://www.semanticweb.org/research-organization#Laboratory
:Laboratory rdf:type owl:Class ;
            rdfs:subClassOf [ rdf:type owl:Restriction ;
                              owl:onProperty :hasResearchGroup ;
                              owl:minQualifiedCardinality "1"^^xsd:nonNegativeInteger ;
                              owl:onClass :ResearchGroup
                            ] ,
                            [ rdf:type owl:Restriction ;
                              owl:onProperty :hasLaboratoryName ;
                              owl:qualifiedCardinality "1"^^xsd:nonNegativeInteger ;
                              owl:onDataRange xsd:string
                            ] ;
            rdfs:comment "A Laboratory is part of a research organization. Each Laboratory has a name and at least one research group"@en ;
            rdfs:label "laboratory"@en .


###  http://www.semanticweb.org/research-organization#Location
:Location rdf:type owl:Class ;
          rdfs:comment "A Location is a spatial region or named place"@en ;
          rdfs:label "location"@en .


###  http://www.semanticweb.org/research-organization#Office
:Office rdf:type owl:Class ;
        rdfs:subClassOf [ rdf:type owl:Restriction ;
                          owl:onProperty :hosts ;
                          owl:someValuesFrom :Employee
                        ] ,
                        [ rdf:type owl:Restriction ;
                          owl:onProperty :hosts ;
                          owl:minQualifiedCardinality "1"^^xsd:nonNegativeInteger ;
                          owl:onClass :Employee
                        ] ;
        rdfs:comment "An Office is a room that hosts one or more employees"@en ;
        rdfs:label "office"@en .


###  http://www.semanticweb.org/research-organization#PostdoctoralFellow
:PostdoctoralFellow rdf:type owl:Class ;
                    rdfs:subClassOf :Employee ,
                                    [ rdf:type owl:Restriction ;
                                      owl:onProperty :isMemberOfLaboratory ;
                                      owl:qualifiedCardinality "1"^^xsd:nonNegativeInteger ;
                                      owl:onClass :Laboratory
                                    ] ,
                                    [ rdf:type owl:Restriction ;
                                      owl:onProperty :isMemberOfResearchGroup ;
                                      owl:qualifiedCardinality "1"^^xsd:nonNegativeInteger ;
                                      owl:onClass :ResearchGroup
                                    ] ;
                    rdfs:comment "An PostdoctoralFellow is an employee that is member of exactly one laboratory and research group"@en ;
                    rdfs:label "postdoctoral fellow"@en .


###  http://www.semanticweb.org/research-organization#ResearchGroup
:ResearchGroup rdf:type owl:Class ;
               rdfs:subClassOf [ rdf:type owl:Restriction ;
                                 owl:onProperty :hasResearchGroupName ;
                                 owl:qualifiedCardinality "1"^^xsd:nonNegativeInteger ;
                                 owl:onDataRange xsd:string
                               ] ;
               rdfs:comment "A Reasearch Group has name and is part of a research organization"@en ;
               rdfs:label "research group"@en .


###  http://www.semanticweb.org/research-organization#ResearchOrganization
:ResearchOrganization rdf:type owl:Class ;
                      rdfs:subClassOf <http://xmlns.com/foaf/0.1/Organization> ,
                                      [ rdf:type owl:Restriction ;
                                        owl:onProperty :hasInstitute ;
                                        owl:someValuesFrom :Institute
                                      ] ;
                      rdfs:comment "A ResearchOrganization is a type of Organization, it makes contracts with employees and consists of more than one institute"@en ;
                      rdfs:label "research organization"@en .


###  http://www.semanticweb.org/research-organization#Researcher
:Researcher rdf:type owl:Class ;
            rdfs:subClassOf :Employee ,
                            [ rdf:type owl:Restriction ;
                              owl:onProperty :isMemberOfLaboratory ;
                              owl:qualifiedCardinality "1"^^xsd:nonNegativeInteger ;
                              owl:onClass :Laboratory
                            ] ,
                            [ rdf:type owl:Restriction ;
                              owl:onProperty :isMemberOfResearchGroup ;
                              owl:qualifiedCardinality "1"^^xsd:nonNegativeInteger ;
                              owl:onClass :ResearchGroup
                            ] ;
            rdfs:comment "A Researcher is person that is an employee and can be a young researcher, a senior researcher or a director. A Researcher is member of one laboratory and one research group"@en ;
            rdfs:label "researcher"@en .


###  http://www.semanticweb.org/research-organization#SeniorResearcher
:SeniorResearcher rdf:type owl:Class ;
                  rdfs:subClassOf :Researcher ;
                  rdfs:comment "A SeniorResearcher is a person that is an Employee and a Researcher"@en ;
                  rdfs:label "senior researcher"@en .


###  http://www.semanticweb.org/research-organization#Technologist
:Technologist rdf:type owl:Class ;
              rdfs:subClassOf :Employee ,
                              [ rdf:type owl:Restriction ;
                                owl:onProperty :isMemberOfLaboratory ;
                                owl:qualifiedCardinality "1"^^xsd:nonNegativeInteger ;
                                owl:onClass :Laboratory
                              ] ,
                              [ rdf:type owl:Restriction ;
                                owl:onProperty :isMemberOfResearchGroup ;
                                owl:qualifiedCardinality "1"^^xsd:nonNegativeInteger ;
                                owl:onClass :ResearchGroup
                              ] ;
              rdfs:comment "A Technologist is a person and an employee, is member of exactly one laboratory and one research group"@en ;
              rdfs:label "technologist"@en .


###  http://www.semanticweb.org/research-organization#YoungResearcher
:YoungResearcher rdf:type owl:Class ;
                 rdfs:subClassOf :Researcher ;
                 rdfs:comment "A YoungResearcher is a person that is an Employee and a Researcher"@en ;
                 rdfs:label "young researcher"@en .


###  http://xmlns.com/foaf/0.1/Organization
<http://xmlns.com/foaf/0.1/Organization> rdf:type owl:Class ;
                                         rdfs:comment "An Organization is a social entity uniting people into a structured group managing shared means to meet some needs, or to pursue collective goals. It can be: Research Organization"@en ;
                                         rdfs:label "organization"@en .


###  http://xmlns.com/foaf/0.1/Person
<http://xmlns.com/foaf/0.1/Person> rdf:type owl:Class ;
                                   rdfs:comment "A person can be: employee (graduate or postdoctoral fellow, young or senior researcher, director, technologist)"@en ;
                                   rdfs:label "person"@en .


#################################################################
#    Individuals
#################################################################

###  http://www.semanticweb.org/research-organization#AIMH
:AIMH rdf:type owl:NamedIndividual ,
               :Laboratory ;
      :hasLaboratoryMember :giovanniBlu ;
      :hasResearchGroup :gorupB ;
      :isLaboratoryOf :unipi ;
      :hasLaboratoryName "Laboratorio AIMH"^^xsd:string .


###  http://www.semanticweb.org/research-organization#antonioPonte
:antonioPonte rdf:type owl:NamedIndividual ,
                       :SeniorResearcher ;
              :hasContractWith :beyondResearch ;
              :isMemberOfLaboratory :AIMH ;
              :hasEmployeeID "456"^^xsd:positiveInteger .


###  http://www.semanticweb.org/research-organization#bari
:bari rdf:type owl:NamedIndividual ,
               :Location ;
      :isLocationOf :edificioB1 .


###  http://www.semanticweb.org/research-organization#beyondResearch
:beyondResearch rdf:type owl:NamedIndividual ,
                         :ResearchOrganization ;
                :makesContractWith :francescoCeleste ,
                                   :giovanniBlu .


###  http://www.semanticweb.org/research-organization#booleLab
:booleLab rdf:type owl:NamedIndividual ,
                   :Laboratory ;
          :hasLaboratoryMember :francescoCeleste ;
          :isLaboratoryOf :unipi ;
          :hasLaboratoryName "Laboratorio Boole" .


###  http://www.semanticweb.org/research-organization#cimecResearch
:cimecResearch rdf:type owl:NamedIndividual ,
                        :ResearchOrganization ;
               :makesContractWith :filippoAllegri ,
                                  :paoloNeri .


###  http://www.semanticweb.org/research-organization#edificioA1
:edificioA1 rdf:type owl:NamedIndividual ,
                     :Building ;
            :hasLocation :pisa ;
            :hasOffice :office00 ;
            :isBuildingOf :unipi .


###  http://www.semanticweb.org/research-organization#edificioA2
:edificioA2 rdf:type owl:NamedIndividual ,
                     :Building ;
            :hasLocation :pisa ;
            :isBuildingOf :unipi .


###  http://www.semanticweb.org/research-organization#edificioB1
:edificioB1 rdf:type owl:NamedIndividual ,
                     :Building ;
            :hasLocation :bari ;
            :isBuildingOf :uniba .


###  http://www.semanticweb.org/research-organization#fabioBruno
:fabioBruno rdf:type owl:NamedIndividual ,
                     :Technologist ;
            :hasContractWith :beyondResearch ;
            :isMemberOfLaboratory :AIMH .


###  http://www.semanticweb.org/research-organization#filippoAllegri
:filippoAllegri rdf:type owl:NamedIndividual ,
                         :SeniorResearcher ;
                :hasContractWith :cimecResearch ;
                :hasEmployeeID "1002"^^xsd:positiveInteger .


###  http://www.semanticweb.org/research-organization#francescoCeleste
:francescoCeleste rdf:type owl:NamedIndividual ,
                           :GraduateFellow ;
                  :hasContractWith :beyondResearch ;
                  :isHostedIn :office00 ;
                  :isMemberOf :unipi ;
                  :isMemberOfLaboratory :booleLab ;
                  :hasEmployeeID "10066"^^xsd:positiveInteger .


###  http://www.semanticweb.org/research-organization#giacomoGiallo
:giacomoGiallo rdf:type owl:NamedIndividual ,
                        :PostdoctoralFellow ;
               :hasContractWith :cimecResearch ;
               :isHostedIn :office02 ;
               :hasEmployeeID "1022"^^xsd:positiveInteger .


###  http://www.semanticweb.org/research-organization#gianniRosa
:gianniRosa rdf:type owl:NamedIndividual ,
                     :YoungResearcher ;
            :hasContractWith :cimecResearch ;
            :hasEmployeeID "12289"^^xsd:positiveInteger .


###  http://www.semanticweb.org/research-organization#giovanniBlu
:giovanniBlu rdf:type owl:NamedIndividual ,
                      :Director ;
             :directs :unipi ;
             :hasContractWith :beyondResearch ;
             :isHostedIn :office01 ;
             :isMemberOf :unipi ;
             :isMemberOfResearchGroup :groupA ;
             :hasEmployeeID "2231"^^xsd:positiveInteger .


###  http://www.semanticweb.org/research-organization#gorupB
:gorupB rdf:type owl:NamedIndividual ,
                 :ResearchGroup ;
        :hasResearchGroupName "Gruppo B0001" .


###  http://www.semanticweb.org/research-organization#groupA
:groupA rdf:type owl:NamedIndividual ,
                 :ResearchGroup ;
        :isResearchGroupOf :booleLab ;
        :hasResearchGroupName "Gruppo A0001" .


###  http://www.semanticweb.org/research-organization#groupC
:groupC rdf:type owl:NamedIndividual ,
                 :ResearchGroup ;
        :isResearchGroupOf :turingLab ;
        :hasResearchGroupName "Gruppo C0001" .


###  http://www.semanticweb.org/research-organization#marioRossi
:marioRossi rdf:type owl:NamedIndividual ,
                     :AdministrativeStaff ;
            :hasContractWith :beyondResearch ;
            :isMemberOf :unipi ;
            :hasEmployeeID "3321"^^xsd:positiveInteger .


###  http://www.semanticweb.org/research-organization#office00
:office00 rdf:type owl:NamedIndividual ,
                   :Office ;
          :hosts :francescoCeleste ,
                 :marioRossi ;
          :isOfficeOf :edificioA1 .


###  http://www.semanticweb.org/research-organization#office01
:office01 rdf:type owl:NamedIndividual ,
                   :Office ;
          :hosts :giovanniBlu ;
          :isOfficeOf :edificioA2 .


###  http://www.semanticweb.org/research-organization#office02
:office02 rdf:type owl:NamedIndividual ,
                   :Office ;
          :hosts :filippoAllegri ,
                 :giacomoGiallo ,
                 :gianniRosa ,
                 :paoloNeri ;
          :isOfficeOf :edificioB1 .


###  http://www.semanticweb.org/research-organization#paoloNeri
:paoloNeri rdf:type owl:NamedIndividual ,
                    :Technologist ;
           :hasContractWith :cimecResearch ;
           :isHostedIn :office02 ;
           :hasEmployeeID "10221"^^xsd:positiveInteger .


###  http://www.semanticweb.org/research-organization#pisa
:pisa rdf:type owl:NamedIndividual ,
               :Location ;
      :isLocationOf :edificioA1 ,
                    :edificioA2 .


###  http://www.semanticweb.org/research-organization#turingLab
:turingLab rdf:type owl:NamedIndividual ,
                    :Laboratory ;
           :hasLaboratoryMember :filippoAllegri ,
                                :giacomoGiallo ;
           :isLaboratoryOf :uniba ;
           :hasLaboratoryName "Laboratorio Turing" .


###  http://www.semanticweb.org/research-organization#uniba
:uniba rdf:type owl:NamedIndividual ,
                :Institute ;
       :hasBuilding :edificioB1 ;
       :hasLaboratory :turingLab ;
       :isInstituteOf :cimecResearch ;
       :hasDate "2004-05-30T09:00:00"^^xsd:dateTime ;
       :hasInstituteID 12227 ;
       :hasInstituteName "Università degli studi di Bari" .


###  http://www.semanticweb.org/research-organization#unipi
:unipi rdf:type owl:NamedIndividual ,
                :Institute ;
       :hasBuilding :edificioA1 ,
                    :edificioA2 ;
       :hasLaboratory :booleLab ;
       :isDirectedBy :giovanniBlu ;
       :isInstituteOf :beyondResearch ;
       :hasDate "2002-05-30T09:00:00"^^xsd:dateTime ;
       :hasInstituteID 1223 ;
       :hasInstituteName "Università degli studi di Pisa" .


#################################################################
#    General axioms
#################################################################

[ rdf:type owl:AllDisjointClasses ;
  owl:members ( :AdministrativeStaff
                :GraduateFellow
                :PostdoctoralFellow
                :Researcher
                :Technologist
              )
] .


[ rdf:type owl:AllDisjointClasses ;
  owl:members ( :Building
                :Employee
                :Institute
                :Laboratory
                :Location
                :Office
                :ResearchGroup
                :ResearchOrganization
              )
] .


[ rdf:type owl:AllDisjointClasses ;
  owl:members ( :Director
                :SeniorResearcher
                :YoungResearcher
              )
] .


[ rdf:type owl:AllDisjointProperties ;
  owl:members ( :hasDate
                :hasID
                :hasName
              )
] .


[ rdf:type owl:AllDisjointProperties ;
  owl:members ( :hasInstituteName
                :hasLaboratoryName
                :hasResearchGroupName
              )
] .


###  Generated by the OWL API (version 4.5.9.2019-02-01T07:24:44Z) https://github.com/owlcs/owlapi
